Db/Examples.lean
@@ -1,0 +1,3 @@
+import Db.Examples.Book
+import Db.Examples.Fish
+import Db.Examples.Member
