Db/Examples/Main.lean
@@ -1,0 +1,4 @@
+import Db.Examples
+
+def main : IO Unit :=
+  BookExample.test
