Db/Interpretation/Basic.lean
@@ -4,6 +4,7 @@ Released under Apache 2.0 license as described in the file LICENSE.
 Authors: Christian Merten
 -/
 import Db.Migration.Basic
+import Db.Migration.Recipe
 
 structure Interpretation (query : Type) where
   fromQuery {d : Database} (names : Std.HashSet d.Name) (q : Query d names) : query
@@ -13,7 +14,7 @@ structure Interpretation (query : Type) where
 class DBMonad (d : Database) (m : Type → Type) where
   /-- Lookup the given query on the database. -/
   lookup {names : Std.HashSet d.Name} (q : Query d names) :
-    m (Array (Std.DHashMap d.Name (fun d ↦ d.dbtype.Value)))
+    m (Array (Std.DHashMap d.Name (fun d ↦ d.column.Value)))
   /-- Insert the given data into the database. Return true if successful, false otherwise. -/
   insert {name : d.Index} (data : d.Insert name) : m Unit
   /-- Delete rows matching the expression. Return number of deleted rows. -/
@@ -23,8 +24,8 @@ class DBMonadWithMigrations (m : Type → Type) where
   [dbMonad (d : Database) : DBMonad d m]
   /- Initialize with given database description. -/
   -- init (d : Database) : m Unit
-  -- this does not work because `Database : Type 1`
-  -- currentDatabase : m Database
+  /-- The current database configuration. -/
+  currentDatabase : m DatabaseRecipe
   /- Execute the given migration. -/
   -- migrate {source target : Database} (migration : source.Migration target) : m Unit
   -- TODO: Replace this with a proper implementation.
