Db/Migration/Recipe.lean
@@ -1,0 +1,82 @@
+/-
+Copyright (c) 2025 Christian Merten. All rights reserved.
+Released under Apache 2.0 license as described in the file LICENSE.
+Authors: Christian Merten
+-/
+import Db.Query.Basic
+
+universe t u
+
+section
+
+variable {α : Type u} {k : Type t} [Hashable k] [BEq k] [LawfulBEq k] [LawfulHashable k]
+
+def Std.HashMap.IndexType (m : Std.HashMap k α) : Type :=
+  Fin m.keys.length
+  deriving Hashable, DecidableEq, Repr, Enum
+
+instance (m : Std.HashMap k α) [ToString k] : ToString m.IndexType where
+  toString (i : Fin _) := toString m.keys[i]
+
+instance (m : Std.HashMap k α) [FromString k] : FromString m.IndexType where
+  fromString s :=
+    -- Can't use `Option` monad, because of universe polymorphism
+    match (FromString.fromString s : Option k) with
+    | some key => List.finIdxOf? key _
+    | none => none
+
+attribute [grind .] Std.HashMap.mem_of_mem_keys
+
+theorem List.Nodup.finIdxOf?_getElem {α : Type u} [BEq α] [LawfulBEq α] {l : List α}
+    (i : Fin l.length) (h : l.Nodup) : l.finIdxOf? l[i] = i := by
+  rw [List.finIdxOf?_eq_some_iff]
+  refine ⟨rfl, fun j hj heq => ?_⟩
+  suffices j = i by grind
+  ext
+  apply List.getElem?_inj j.isLt h
+  grind
+
+-- TODO: generalise by adding a `LawfulFromToString` class
+instance (m : Std.HashMap String α) : Indexing m.IndexType where
+  fromString_toString (i : Fin _) := by
+    show List.finIdxOf? m.keys[i] _ = _
+    exact Std.HashMap.nodup_keys.finIdxOf?_getElem _
+
+end
+
+/--
+The minimal data required for defining a table. This is less convenient to work with, because
+it does not contain an explicit indexing type. But `Table : Type 1`, which
+causes universe issues with monads.
+-/
+structure TableRecipe : Type where
+  columns : Std.HashMap String Column
+  deriving Repr
+
+/--
+The minimal data required for defining a database. This is less convenient to work with, because
+it does not contain an explicit indexing type. But `Database : Type 1`, which
+causes universe issues with monads.
+-/
+structure DatabaseRecipe : Type where
+  tables : Std.HashMap String TableRecipe
+  deriving Repr
+
+def TableRecipe.Index (recipe : TableRecipe) : Type :=
+  recipe.columns.IndexType
+  deriving Indexing
+
+def DatabaseRecipe.Index (recipe : DatabaseRecipe) : Type :=
+  recipe.tables.IndexType
+  deriving Indexing
+
+/-- A reconstructed table from a table recipe. -/
+def TableRecipe.table (recipe : TableRecipe) : Table where
+  Index := recipe.Index
+  columns (i : Fin _) := recipe.columns[recipe.columns.keys[i]]'(by grind)
+
+/-- A reconstructed database from a database recipe. -/
+def DatabaseRecipe.table (recipe : DatabaseRecipe) : Database where
+  Index := recipe.Index
+  tables (i : Fin _) :=
+    recipe.tables[recipe.tables.keys[i]]'(by grind) |>.table
